wip: Two-staged processor refinement proof

examples/ProcTwoStDec.v
@@ -5,7 +5,7 @@ Require Import Kami.Syntax Kami.Semantics Kami.RefinementFacts Kami.Renaming Kam
 Require Import Kami.Renaming Kami.Inline Kami.InlineFacts.
 Require Import Kami.Decomposition Kami.Notations Kami.Tactics.
 Require Import Ex.MemTypes Ex.NativeFifo Ex.MemAtomic.
-Require Import Ex.SC Ex.ProcTwoStage Ex.ProcDec Ex.ProcDecInl Ex.ProcDecInv.
+Require Import Ex.SC Ex.ProcDec Ex.ProcTwoStage Ex.ProcTwoStInl Ex.ProcTwoStInv.
 Require Import Eqdep.
 
 Set Implicit Arguments.
@@ -42,11 +42,66 @@ Section ProcTwoStDec.
       "execNm" |-> "execNm"; ||.
   Hint Unfold p2st_pdec_ruleMap: MethDefs.
 
-  (* TODO: p2st_pdec_regMap *)
-  
-  Theorem p2st_refines_pdec: p2st <<== pdec.
+  Definition p2st_pdec_regMap (r: RegsT): RegsT :=
+    (mlet pcv : (Bit addrSize) <- r of "pc";
+       mlet rfv : (Vector (Data lgDataBytes) rfIdx) <- r of "rf";
+       mlet d2eeltv : d2eElt opIdx addrSize lgDataBytes rfIdx <- r of "d2e"--"elt";
+       mlet d2efv : Bool <- r of "d2e"--"full";
+       mlet e2deltv : Bit addrSize <- r of "e2d"--"elt";
+       mlet e2dfv : Bool <- r of "e2d"--"full";
+       mlet curv : d2eElt opIdx addrSize lgDataBytes rfIdx <- r of "curInfo";
+       mlet fstallv : Bool <- r of "fetchStall";
+       mlet stallv : Bool <- r of "stall";
+       (["stall" <- existT _ _ stallv]
+        +["fetchStall" <- existT _ _ fstallv]
+        +["fetched" <- existT _ (SyntaxKind (DecInstK opIdx addrSize lgDataBytes rfIdx))
+                    (curv ``"instDec")]
+        +["fetch" <- existT _ (SyntaxKind Bool) (negb d2efv)]
+        +["rf" <- existT _ _ rfv]
+        +["pc" <- existT _ (SyntaxKind (Bit addrSize))
+               (if d2efv then d2eeltv ``"curPc"
+                else if e2dfv then e2deltv
+                     else pcv)])%fmap)%mapping.
+  Hint Unfold p2st_pdec_regMap: MapDefs.
+
+  Theorem p2st_refines_pdec:
+    p2st <<== pdec.
   Proof.
-    admit.
+    kinline_left im.
+    kdecompose_nodefs p2st_pdec_regMap p2st_pdec_ruleMap.
+
+    kinv_add p2st_inv_ok.
+    kinv_add_end.
+    
+    kinvert.
+
+    (* 1: "modifyPc" proved *)
+
+    Focus 2.
+
+    kinv_action_dest.
+    destruct Hr; kinv_red.
+    kinv_regmap_red.
+    kinv_constr.
+
+    
+
+    kinv_eq.
+
+      
+
+    - (* "reqInstFetch" needs an invariant about "d2e" emptiness, 
+       * since "d2e.empty" is mapped to "fetch" *)
+      admit.
+
+    - (* "repInstFetch" needs invariants about:
+       * 1) "d2e.empty" is mapped to "fetch"
+       * 2) decoded instruction = curInfov
+       * 3) pc mismatch: x2 = x2 + 1?
+       * --> pc is speculated in "repInstFetch" in the decode module
+       * --> need to think about "pc" mapping
+       *)
+      
   Qed.
 
 End ProcTwoStDec.
