examples/ProcTwoStInl.v
@@ -1,0 +1,30 @@
+Require Import Kami.Syntax Kami.Semantics Kami.RefinementFacts Kami.Renaming Kami.Wf.
+Require Import Kami.Inline Kami.InlineFacts Kami.Tactics.
+Require Import Ex.SC Ex.ProcTwoStage.
+
+Set Implicit Arguments.
+
+Section Inlined.
+  Variables opIdx addrSize fifoSize lgDataBytes rfIdx: nat.
+
+  Variable dec: DecT opIdx addrSize lgDataBytes rfIdx.
+  Variable execState: ExecStateT opIdx addrSize lgDataBytes rfIdx.
+  Variable execNextPc: ExecNextPcT opIdx addrSize lgDataBytes rfIdx.
+
+  Variables opLd opSt opTh: ConstT (Bit opIdx).
+
+  Definition p2st := p2st dec execState execNextPc opLd opSt opTh.
+  Hint Unfold p2st: ModuleDefs. (* for kinline_compute *)
+
+  Definition p2stInl: Modules * bool.
+  Proof.
+    remember (inlineF p2st) as inlined.
+    kinline_compute_in Heqinlined.
+    match goal with
+    | [H: inlined = ?m |- _] =>
+      exact m
+    end.
+  Defined.
+
+End Inlined.
+
