examples/ProcTwoStInv.v
@@ -1,0 +1,89 @@
+Require Import Bool String List.
+Require Import Lib.CommonTactics Lib.ilist Lib.Word.
+Require Import Lib.Struct Lib.StructNotation Lib.StringBound Lib.FMap Lib.StringEq Lib.Indexer.
+Require Import Kami.Syntax Kami.Semantics Kami.RefinementFacts Kami.Renaming Kami.Wf.
+Require Import Kami.Renaming Kami.Specialize Kami.Inline Kami.InlineFacts Kami.Decomposition.
+Require Import Kami.Tactics Kami.Notations.
+Require Import Ex.MemTypes Ex.SC Ex.NativeFifo Ex.MemAtomic Ex.ProcTwoStage Ex.ProcTwoStInl.
+Require Import Eqdep ProofIrrelevance.
+
+Set Implicit Arguments.
+
+Section Invariants.
+  Variables opIdx addrSize fifoSize lgDataBytes rfIdx: nat.
+
+  Variable dec: DecT opIdx addrSize lgDataBytes rfIdx.
+  Variable execState: ExecStateT opIdx addrSize lgDataBytes rfIdx.
+  Variable execNextPc: ExecNextPcT opIdx addrSize lgDataBytes rfIdx.
+
+  Variables opLd opSt opTh: ConstT (Bit opIdx).
+  Hypothesis (HldSt: (if weq (evalConstT opLd) (evalConstT opSt) then true else false) = false).
+
+  Definition RqFromProc := MemTypes.RqFromProc lgDataBytes (Bit addrSize).
+  Definition RsToProc := MemTypes.RsToProc lgDataBytes.
+
+  Definition p2stInl := p2stInl dec execState execNextPc opLd opSt opTh.
+
+  Record p2st_inv (o: RegsT) : Prop :=
+    { pcv : fullType type (SyntaxKind (Bit addrSize));
+      Hpcv : M.find "pc"%string o = Some (existT _ _ pcv);
+      fstallv : fullType type (SyntaxKind Bool);
+      Hfstallv : M.find "fetchStall"%string o = Some (existT _ _ fstallv);
+      fepochv : fullType type (SyntaxKind Bool);
+      Hfepochv : M.find "fEpoch"%string o = Some (existT _ _ fepochv);
+      rfv : fullType type (SyntaxKind (Vector (Data lgDataBytes) rfIdx));
+      Hrfv : M.find "rf"%string o = Some (existT _ _ rfv);
+
+      d2eeltv : fullType type (SyntaxKind (d2eElt opIdx addrSize lgDataBytes rfIdx));
+      Hd2eeltv : M.find "d2e"--"elt"%string o = Some (existT _ _ d2eeltv);
+      d2efullv : fullType type (SyntaxKind Bool);
+      Hd2efullv : M.find "d2e"--"full"%string o = Some (existT _ _ d2efullv);
+
+      e2deltv : fullType type (SyntaxKind (Bit addrSize));
+      He2deltv : M.find "e2d"--"elt"%string o = Some (existT _ _ e2deltv);
+      e2dfullv : fullType type (SyntaxKind Bool);
+      He2dfullv : M.find "e2d"--"full"%string o = Some (existT _ _ e2dfullv);
+
+      stallv : fullType type (SyntaxKind Bool);
+      Hstallv : M.find "stall"%string o = Some (existT _ _ stallv);
+      eepochv : fullType type (SyntaxKind Bool);
+      Heepochv : M.find "eEpoch"%string o = Some (existT _ _ eepochv);
+      curInfov : fullType type (SyntaxKind (d2eElt opIdx addrSize lgDataBytes rfIdx));
+      HcurInfov : M.find "curInfo"%string o = Some (existT _ _ curInfov)
+    }.
+
+  Ltac p2st_inv_old :=
+    try match goal with
+        | [H: p2st_inv _ |- _] => destruct H
+        end;
+    kinv_red.
+  
+  Ltac p2st_inv_new :=
+    econstructor; (* let's prove that the invariant holds for the next state *)
+    try (findReify; (reflexivity || eassumption); fail);
+    kregmap_clear. (* for improving performance *)
+
+  Ltac p2st_inv_tac := p2st_inv_old; p2st_inv_new.
+
+  Lemma p2st_inv_ok':
+    forall init n ll,
+      init = initRegs (getRegInits (fst p2stInl)) ->
+      Multistep (fst p2stInl) init n ll ->
+      p2st_inv n.
+  Proof.
+    admit.
+  Qed.
+  
+  Lemma p2st_inv_ok:
+    forall o,
+      reachable o (fst p2stInl) ->
+      p2st_inv o.
+  Proof.
+    intros; inv H; inv H0.
+    eapply p2st_inv_ok'; eauto.
+  Qed.
+
+End Invariants.
+
+Hint Unfold RqFromProc RsToProc: MethDefs.
+
